Simple Enc protocol automated

protocols/SimplePingEncProtocolsAutomated.v
@@ -37,87 +37,11 @@ Require IdealWorld RealWorld.
 Import IdealWorld.IdealNotations.
 Import RealWorld.RealWorldNotations.
 
+Require
+  SimplePingProtocol
+  SimpleEncProtocol.
+
 Set Implicit Arguments.
-
-(* User ids *)
-Definition A : user_id   := 0.
-Definition B : user_id   := 1.
-
-Section IdealProtocol.
-  Import IdealWorld.
-
-  Definition CH__A2B : channel_id := 0.
-
-  Definition PERMS__a := $0 $+ (CH__A2B, {| read := true; write := true |}). (* writer *)
-  Definition PERMS__b := $0 $+ (CH__A2B, {| read := true; write := false |}). (* reader *)
-
-  Definition mkiU (cv : channels) (p__a p__b : cmd (Base Nat)): universe Nat :=
-    {| channel_vector := cv
-     ; users := $0
-         $+ (A,   {| perms    := PERMS__a ; protocol := p__a |})
-         $+ (B,   {| perms    := PERMS__b ; protocol := p__b |})
-    |}.
-
-  Definition ideal_univ_start :=
-    mkiU ($0 $+ (CH__A2B, []))
-         (* user A *)
-         ( n <- Gen
-         ; _ <- Send (Content n) CH__A2B
-         ; Return n)
-         (* user B *)
-         ( m <- @Recv Nat CH__A2B
-         ; ret (extractContent m)).
-
-End IdealProtocol.
-
-Section RealProtocolParams.
-  Import RealWorld.
-
-  Definition KID1 : key_identifier := 0.
-
-  Definition KEY1  := MkCryptoKey KID1 Signing AsymKey.
-  Definition KEYS  := $0 $+ (KID1, KEY1).
-
-  Definition A__keys := $0 $+ (KID1, true).
-  Definition B__keys := $0 $+ (KID1, false).
-End RealProtocolParams.
-
-Section RealProtocol.
-  Import RealWorld.
-
-  Definition mkrU (mycs1 mycs2 : my_ciphers) (froms1 froms2 : recv_nonces)
-                  (sents1 sents2 : sent_nonces) (cur_n1 cur_n2 : nat)
-                  (msgs1 msgs2 : queued_messages) (cs : ciphers)
-                  (p__a p__b : user_cmd (Base Nat)) (adv : user_data Unit) : universe Nat Unit :=
-    {| users := $0
-         $+ (A, {| key_heap := A__keys ; protocol := p__a ; msg_heap := msgs1 ; c_heap := mycs1
-                 ; from_nons := froms1 ; sent_nons := sents1 ; cur_nonce := cur_n1 |})
-         $+ (B, {| key_heap := B__keys ; protocol := p__b ; msg_heap := msgs2 ; c_heap := mycs2
-                 ; from_nons := froms2 ; sent_nons := sents2 ; cur_nonce := cur_n2 |})
-     ; adversary        := adv
-     ; all_ciphers      := cs
-     ; all_keys         := KEYS
-    |}.
-
-  Definition real_univ_start cs mycs1 mycs2 cur_n1 cur_n2 :=
-    mkrU mycs1 mycs2 [] [] [] [] cur_n1 cur_n2 [] [] cs
-         (* user A *)
-         ( n  <- Gen
-         ; c  <- Sign KID1 B (message.Content n)
-         ; _  <- Send B c
-         ; Return n)
-
-         (* user B *)
-         ( c  <- @Recv Nat (Signed KID1 true)
-         ; v  <- Verify KID1 c
-         ; ret (if fst v
-                then match snd v with
-                     | message.Content p => p
-                     | _                 => 0
-                     end
-                else 1)).
-  
-End RealProtocol.
 
 Import SimulationAutomation.
 
@@ -127,6 +51,8 @@ End Foo.
 Module Import SN := SetNotations(Foo).
 
 Module SimplePingProtocolSecure <: AutomatedSafeProtocol.
+
+  Import SimplePingProtocol.
 
   Definition t__hon := Nat.
   Definition t__adv := Unit.
@@ -235,3 +161,114 @@ Module SimplePingProtocolSecure <: AutomatedSafeProtocol.
 
 
 End SimplePingProtocolSecure.
+
+Module SimpleEncProtocolSecure <: AutomatedSafeProtocol.
+
+  Import SimpleEncProtocol.
+
+  Definition t__hon := Nat.
+  Definition t__adv := Unit.
+  Definition b := tt.
+  Definition iu0  := ideal_univ_start.
+  Definition ru0  := real_univ_start $0 [] [] 0 0 startAdv.
+
+  Import Gen ModelCheck Invariant Tacs SetLemmas.
+
+  Hint Unfold t__hon t__adv b ru0 iu0 ideal_univ_start mkiU real_univ_start mkrU : core.
+
+  Lemma safe_invariant :
+    invariantFor
+      {| Initial := {(ru0, iu0)}; Step := @step t__hon t__adv  |}
+      (lift_fst honest_cmds_safe).
+  Proof.
+    eapply Invariant.invariant_weaken.
+
+    - apply multiStepClosure_ok; simpl.
+      gen1.
+      gen1.
+      gen1.
+      gen1.
+      gen1.
+      gen1.
+      gen1.
+      gen1.
+
+    - intros.
+      simpl in *.
+      sets_invert; unfold lift_fst;
+        split_ex; simpl in *; subst; solve_honest_actions_safe;
+          clean_map_lookups; eauto 8.
+
+      Unshelve.
+      all:eauto.
+  Qed.
+
+  Lemma U_good : @universe_starts_sane _ Unit b ru0.
+  Proof.
+    autounfold;
+      unfold universe_starts_sane; simpl.
+    repeat (apply conj); intros; eauto.
+    - solve_perm_merges; eauto.
+    - econstructor.
+    - unfold AdversarySafety.keys_honest, KEYS; rewrite Forall_natmap_forall; intros.
+      econstructor; simpl.
+      rewrite !findUserKeys_add_reduce, findUserKeys_empty_is_empty; eauto.
+      solve_perm_merges.
+    - unfold lameAdv; simpl; eauto.
+  Qed.
+
+  Lemma univ_ok_start : universe_ok ru0.
+  Proof.
+    autounfold; econstructor; eauto.
+  Qed.
+
+  Lemma adv_univ_ok_start : adv_universe_ok ru0.
+  Proof.
+    autounfold; unfold adv_universe_ok; eauto.
+    unfold keys_and_permissions_good.
+    pose proof (adversary_is_lame_adv_univ_ok_clauses U_good).
+
+    intuition eauto;
+      simpl in *.
+
+    - unfold KEYS in *; solve_simple_maps; eauto.
+    - rewrite Forall_natmap_forall; intros.
+      solve_simple_maps; simpl;
+        unfold permission_heap_good, KEYS, A__keys, B__keys; intros;
+          solve_simple_maps; eauto.
+
+    - unfold user_cipher_queues_ok.
+      rewrite Forall_natmap_forall; intros.
+      cases (A ==n k); cases (B ==n k);
+        subst; clean_map_lookups; simpl in *; econstructor; eauto.
+
+    - unfold honest_nonces_ok; intros.
+      unfold honest_nonce_tracking_ok.
+
+      destruct (u_id ==n A); destruct (u_id ==n B);
+        destruct (rec_u_id ==n A); destruct (rec_u_id ==n B);
+          subst; try contradiction; try discriminate; clean_map_lookups; simpl;
+            repeat (apply conj); intros; clean_map_lookups; eauto.
+
+    - unfold honest_users_only_honest_keys; intros.
+      destruct (u_id ==n A);
+        destruct (u_id ==n B);
+        subst;
+        simpl in *;
+        clean_map_lookups;
+        rewrite !findUserKeys_add_reduce, findUserKeys_empty_is_empty;
+        eauto;
+        simpl in *;
+        solve_perm_merges;
+        solve_concrete_maps;
+        solve_simple_maps;
+        eauto.
+  Qed.
+  
+  Lemma universe_starts_safe : universe_ok ru0 /\ adv_universe_ok ru0.
+  Proof.
+    repeat (simple apply conj);
+      eauto using univ_ok_start, adv_univ_ok_start.
+  Qed.
+
+End SimpleEncProtocolSecure.
